the fixpoint of a (dependent) function.
- also, adding universe annotations. Note that Eff is not truely
  a monad because it is expansive (in universe terms), that means
  that you can not have terms of type `Eff eff (Eff eff a)` because
  the universe of `m a` > the unverse of `a`.

theories/Eff.v
@@ -1,35 +1,42 @@
-Section Eff.
-  Variable eff : Type -> Type.
+Set Universe Polymorphism.
 
-  Inductive EffF (Eff : Type) (T : Type) : Type :=
+Require Import Coq.Classes.Morphisms.
+Require Import Coq.Classes.RelationClasses.
+Require Import Setoid.
+
+Section Eff.
+  Polymorphic Universes u u'.
+  Variable eff : Type@{u} -> Type@{u'}.
+
+  Inductive EffF (Eff : Type@{u'}) (T : Type@{u}) : Type@{u'} :=
   | retF (_ : T)
-  | interactF {A} (_ : eff A) (_ : A -> Eff)
+  | interactF {A : Type@{u}} (_ : eff A) (_ : A -> Eff)
   | delayF (_ : Eff).
 
   Arguments retF {_ _} _.
   Arguments interactF {_ _ _} _ _.
   Arguments delayF {_ _} _.
 
-  CoInductive Eff (T : Type) : Type :=
+  CoInductive Eff (T : Type@{u}) : Type@{u'} :=
   | do (_ : EffF (Eff T) T).
 
   Arguments do {_} _.
 
-  Definition getEff {T} (x : Eff T) : EffF (Eff T) T :=
+  Definition getEff {T : Type@{u}} (x : Eff T) : EffF (Eff T) T :=
     match x with
     | do y => y
     end.
 
-  Definition ret {T} (x : T) : Eff T :=
+  Definition ret {T : Type@{u}} (x : T) : Eff T :=
     do (retF x).
 
-  Definition interact {T U} (x : eff T) (k : T -> Eff U) : Eff U :=
+  Definition interact {T U : Type@{u}} (x : eff T) (k : T -> Eff U) : Eff U :=
     do (interactF x k).
 
-  Definition delay {T} (x : Eff T)  : Eff T :=
+  Definition delay {T : Type@{u}} (x : Eff T)  : Eff T :=
     do (delayF x).
 
-  Theorem getEff_eq : forall {T} (x : Eff T),
+  Theorem getEff_eq : forall {T : Type@{u}} (x : Eff T),
       x = match getEff x with
           | retF v => ret v
           | interactF e k => interact e k
@@ -40,7 +47,7 @@ Section Eff.
   Defined.
 
   Section bind.
-    Context {A B : Type} (k : A -> Eff B).
+    Context {A B : Type@{u}} (k : A -> Eff B).
 
     CoFixpoint bind' (f : Eff A) : Eff B :=
       match getEff f with
@@ -50,8 +57,28 @@ Section Eff.
       end.
   End bind.
 
-  Definition bind {A B} (f : Eff A) (k : A -> Eff B) : Eff B :=
+  Definition bind {A B : Type@{u}} (f : Eff A) (k : A -> Eff B) : Eff B :=
     bind' k f.
+
+  Definition delayBind {t u : Type@{u}} (e : Eff t) (k : t -> Eff u) : Eff u :=
+    match getEff e with
+    | retF v => delay (k v)
+    | interactF e k' =>
+      interact e (fun x => bind (k' x) k)
+    | delayF v => delay (bind v k)
+    end.
+
+  Lemma delayBind_ret : forall {T U} v (k : T -> Eff U),
+      delayBind (ret v) k = delay (k v).
+  Proof. Admitted.
+
+  Lemma delayBind_delay : forall {T U} (v : Eff T) (k : T -> Eff U),
+      delayBind (delay v) k = bind v k.
+  Proof. Admitted.
+
+  Lemma delayBind_interact : forall {T U V} e (k : T -> Eff U) (k' : U -> Eff V),
+      delayBind (interact e k) k' = interact e (fun x => bind (k x) k').
+  Proof. Admitted.
 
   (* I should use paco to define this *)
   CoInductive Eff_eq {T} : Eff T -> Eff T -> Prop :=
@@ -70,11 +97,60 @@ Section Eff.
   | sim_delay : forall a b, Eff_sim a b ->
                        Eff_sim (delay a) (delay b).
 
+  Global Instance Reflexive_Eff_eq {T} : Reflexive (@Eff_eq T).
+  Admitted.
+  Global Instance Symmetric_Eff_eq {T} : Symmetric (@Eff_eq T).
+  Admitted.
+  Global Instance Transitive_Eff_eq {T} : Transitive (@Eff_eq T).
+  Admitted.
+
+  Global Instance Proper_Eff_eq_impl {T}
+  : Proper (@Eff_eq T --> @Eff_eq T ==> Basics.impl) (@Eff_eq _).
+  Proof. red. red. red. red. intros.
+         etransitivity; [ apply H | ].
+         etransitivity; [ eapply H1 | eapply H0 ].
+  Defined.
+
+  Global Instance Proper_Eff_eq_iff {T}
+  : Proper (@Eff_eq T --> @Eff_eq T ==> iff) (@Eff_eq _).
+  Proof. red. red. red. intros.
+         split; eapply Proper_Eff_eq_impl;
+           solve [ assumption | symmetry; assumption ].
+  Defined.
+
+  Global Instance Reflexive_Eff_sim {T} : Reflexive (@Eff_sim T).
+  Admitted.
+  Global Instance Symmetric_Eff_sim {T} : Symmetric (@Eff_sim T).
+  Admitted.
+  Global Instance Transitive_Eff_sim {T} : Transitive (@Eff_sim T).
+  Admitted.
+
+  Global Instance Subrelation_Eff_sim_Eff_eq {T}
+  : subrelation (@Eff_eq T) (@Eff_sim T).
+  Admitted.
+
+  Global Instance Proper_bind' {T U}
+  : Proper (pointwise_relation T (@Eff_eq U) ==> @Eff_eq T ==> (@Eff_eq U)) bind'.
+  Admitted.
+
+  Global Instance Proper_bind {T U}
+  : Proper (@Eff_eq T ==> pointwise_relation T (@Eff_eq U) ==> (@Eff_eq U)) bind.
+  Admitted.
+
+  Global Instance Proper_delayBind {T U}
+  : Proper (@Eff_eq T ==> pointwise_relation T (@Eff_eq U) ==> (@Eff_eq U)) delayBind.
+  Admitted.
+
+  Global Instance Proper_delay {T}
+  : Proper (@Eff_eq T ==> @Eff_eq T) delay.
+  Admitted.
+
 End Eff.
 
 
 Arguments bind {_ _ _} _ _.
 Arguments bind' {_ _ _} _ _.
+Arguments delayBind {_ _ _} _ _.
 Arguments interactF {_ _ _ _} _ _.
 Arguments interact {_ _ _} _ _.
 Arguments retF {_ _ _} _.
@@ -82,6 +158,7 @@ Arguments ret {_ _} _.
 Arguments delayF {_ _ _} _.
 Arguments delay {_ _} _.
 Arguments getEff {_ _} _.
+Arguments getEff_eq {_ _} _.
 
 (** Interpretation of effects *)
 
@@ -95,39 +172,29 @@ Section interp.
     match getEff c with
     | retF x => ret x
     | interactF e k =>
-      match getEff (do _ e) with
-      | retF v => delay (interp (k v))
-      | interactF e k' =>
-        interact e (fun x => bind (k' x) (fun y => interp (k y)))
-      | delayF v => delay (@bind' _ _ _ (fun x => interp (k x)) v)
-      end
+      delayBind (do _ e) (fun x => interp (k x))
     | delayF x => delay (interp x)
     end.
-
-
 
   Lemma interp_ret : forall {T} (v : T),
       interp (ret v) = ret v.
   Proof.
     intros.
     rewrite getEff_eq.
-    rewrite (getEff_eq _ (interp (ret v))).
+    rewrite (getEff_eq (interp (ret v))).
     reflexivity.
   Defined.
 
-  (* This doesn't preserve stuttering *)
   Lemma interp_interact : forall {a b} (e : eff a) (k : a -> Eff eff b),
       interp (interact e k) =
-      bind (do _ e) (fun x => interp (k x)).
+      delayBind (do _ e) (fun x => interp (k x)).
   Proof.
     intros.
     rewrite getEff_eq. symmetry. rewrite getEff_eq. symmetry.
     simpl.
-    destruct (getEff (do a e)); simpl.
-    { admit. }
-    { reflexivity. }
-    { reflexivity. }
-  Admitted.
+    destruct (delayBind (do a e) (fun x : a => interp (k x))).
+    reflexivity.
+  Defined.
 
   Lemma interp_delay : forall {a} (k : Eff eff a),
       interp (delay k) = delay (interp k).
@@ -157,24 +224,30 @@ Section inj.
 
   Variable eff eff' : Type -> Type.
 
-  CoFixpoint injL {T} (c : Eff eff T) : Eff (both eff eff') T :=
-    match getEff c with
-    | retF x => ret x
-    | interactF e k => interact (bleft e) (fun x => injL (k x))
-    | delayF x => delay (injL x)
-    end.
+  Definition injL {T} (c : Eff eff T) : Eff (both eff eff') T :=
+    interp (fun _ e => interact (bleft e) (@ret _ _)) c.
 
-  CoFixpoint injR {T} (c : Eff eff' T) : Eff (both eff eff') T :=
-    match getEff c with
-    | retF x => ret x
-    | interactF e k => interact (bright e) (fun x => injR (k x))
-    | delayF x => delay (injR x)
-    end.
+  Definition injR {T} (c : Eff eff' T) : Eff (both eff eff') T :=
+    interp (fun _ e => interact (bright e) (@ret _ _)) c.
 
 End inj.
 
 Arguments injL {_} _ {_} _.
 Arguments injR {_ _} _ _.
+
+(* the empty effect *)
+Section nothingE.
+  Inductive nothing : Type -> Type := .
+End nothingE.
+
+(* the output effect *)
+Section outputE.
+  Variable t : Type.
+  Inductive out : Type -> Type :=
+  | outE : t -> out t.
+End outputE.
+
+Arguments outE {_} _.
 
 (* the fixpoint effect *)
 Section Fix.
@@ -186,41 +259,41 @@ Section Fix.
 
   Variable eff : Type -> Type.
 
-  (** Begin a bunch of variants to try to implement mfix *)
-
   Section mfix.
     Variable f : Eff (both eff fixpoint) a.
 
-    CoFixpoint finterp_then
-           {T b : Type} (k' : T -> Eff eff b)
-               (c : Eff (both eff fixpoint) T) : Eff eff b :=
+    CoFixpoint finterp {T : Type}
+               (c : Eff (both eff fixpoint) T)
+    : Eff eff T :=
       match getEff c with
-      | retF x => delay (k' x)
+      | retF x => ret x
       | interactF (bleft e) k =>
-        interact e (fun x => finterp_then k' (k x))
+        interact e (fun x => finterp (k x))
       | interactF (bright e) k =>
-        delay (finterp_then k' (bind' (fun x => k match e with
-                                        | rec => x
-                                        end) f))
-      | delayF x => delay (finterp_then k' x)
+        delay (finterp (bind' (fun x => k match e with
+                                       | rec => x
+                                       end) f))
+      | delayF x => delay (finterp x)
       end.
 
-    Definition mfix : Eff eff a := finterp_then ret f.
+    Definition mfix : Eff eff a := finterp f.
+
+    Definition go (mfix : Eff eff a)
+               T (X : both eff fixpoint T) : Eff eff T :=
+      match X with
+      | bleft e => interact e ret
+      | bright f0 =>
+        match f0 with
+        | rec => mfix
+        end
+      end.
+
+
+    Theorem mfix_unfold :
+      mfix = interp (go mfix) f.
+    Proof. Admitted.
+
   End mfix.
-
-  Definition go (mfix : Eff eff a)
-    T (X : both eff fixpoint T) : Eff eff T :=
-    match X with
-    | bleft e => interact e ret
-    | bright f0 =>
-      match f0 with
-      | rec => mfix
-      end
-    end.
-
-  Theorem mfix_unfold : forall f,
-      mfix f = interp (go (mfix f)) f.
-  Proof. Admitted.
 
   Theorem mfix_ret : forall v, mfix (ret v) = ret v.
   Proof. Admitted.
@@ -228,6 +301,71 @@ Section Fix.
 End Fix.
 
 Arguments mfix {_} _.
+
+
+Section FixF.
+
+  Variable a : Type.
+  Variable b : a -> Type.
+
+  Inductive fixpointF : Type -> Type :=
+  | callF : forall x : a, fixpointF (b x).
+
+  Variable eff : Type -> Type.
+
+  Section mfix.
+    Variable f : forall x : a, Eff (both eff fixpointF) (b x).
+
+    CoFixpoint finterpF {T : Type}
+               (c : Eff (both eff fixpointF) T)
+    : Eff eff T :=
+      match getEff c with
+      | retF x => ret x
+      | interactF (bleft e) k =>
+        interact e (fun x => finterpF (k x))
+      | interactF (bright e) k =>
+        match e in fixpointF X return (X -> _) -> _ with
+        | callF x => fun k =>
+          delay (finterpF (bind (f x) k))
+        end k
+      | delayF x => delay (finterpF x)
+      end.
+
+    Definition mfixF (x : a) : Eff eff (b x) := finterpF (f x).
+
+    Definition goF
+               T (X : both eff fixpointF T) : Eff eff T :=
+      match X with
+      | bleft e => interact e ret
+      | bright f0 =>
+        match f0 with
+        | callF x => mfixF x
+        end
+      end.
+
+    Theorem mfixF_unfold : forall x,
+      mfixF x = interp goF (f x).
+    Proof. Admitted.
+
+  End mfix.
+
+  Theorem mfixF_ret : forall v x, mfixF (fun x => ret (v x)) x = ret (v x).
+  Proof. Admitted.
+
+End FixF.
+
+
+Arguments callF {_ _} _.
+
+(* mfix Demo *)
+(* This doesn't work due to universes, it looks like you need a separate
+   fixpoint operator for functions.
+ *)
+Definition count_up : Eff (out nat) False :=
+  mfixF nat (fun _ : nat => False) (out nat)
+        (fun n : nat =>
+           interact (bleft (outE n))
+                    (fun _ : nat => interact (bright (callF (n + 1))) ret)) 0.
 
 (* the state effect *)
 Section stateE.
@@ -241,10 +379,6 @@ End stateE.
 Arguments Get {_}.
 Arguments Put {_} _.
 
-(* the empty effect *)
-Section nothingE.
-  Inductive nothing : Type -> Type := .
-End nothingE.
 
 (** Testing *)
 Definition trial : Eff nothing False :=
@@ -261,21 +395,33 @@ Section diverge.
 
 End diverge.
 
-Require Import Setoid.
+Lemma delayBind_diverge : forall t u eff (k : t -> Eff eff u),
+    Eff_eq eff (delayBind (diverge t) k) (bind (diverge t) k).
+Proof.
+  intros. cofix rec.
+  rewrite diverge_eq.
+  rewrite (getEff_eq (delayBind (delay _) _)).
+  rewrite (getEff_eq (bind (delay _) _)).
+  simpl.
+  constructor. reflexivity.
+Defined.
+
+Lemma bind_diverge : forall t u eff (k : t -> Eff eff u),
+    Eff_eq eff (bind (diverge t) k) (diverge u).
+Proof.
+  intros. cofix rec.
+  rewrite diverge_eq.
+  rewrite (getEff_eq (bind (delay _) _)).
+  rewrite (getEff_eq (diverge u)).
+  simpl.
+  constructor. eapply rec.
+Defined.
 
 Goal Eff_eq _ trial (diverge _).
   cofix rec.
   unfold trial.
   rewrite mfix_unfold.
   rewrite interp_interact. simpl go.
-  rewrite mfix_unfold. rewrite interp_interact.
-  Eval compute in fun f => getEff (mfix nothing f ret).
-
-  rewrite (getEff_eq _ (interp (go _ _ _) _)).
-
-
-  simpl.
-  rewrite (getEff_eq _ (diverge False)). simpl.
-
-
-Admitted.
+  change (mfix nothing (interact (bright (Top.rec False)) ret)) with trial.
+  rewrite rec. rewrite delayBind_diverge. rewrite bind_diverge. reflexivity.
+Admitted. (* need to do paco reasoning *)
